## Prove 

已知:
$$
\begin{aligned}
  f[j](n - j) - \sum_{k = j}^{n - 1} f[k] \leq r \\ 
  f[j - 1](n - j + 1) - \sum_{k = j - 1}^{n - 1}f[k] > r \\ 
  f[j - 1] > f[j]
\end{aligned}
$$

欲证：
$$
f[j - 1] > f[j] + ⌊\frac{r'}{n - j}⌋
$$
其中
$$
r' = r + \sum_{k = j}^{n - 1} f[k] - f[j](n - j)
$$

代入：
$$
\begin{aligned}
  f[j] + ⌊\frac{r'}{n - j}⌋ &= f[j] + ⌊\frac{r + \sum_{k = j}^{n - 1} f[k]}{n - j} - f[j]⌋ \\ 
  &= f[j] + ⌊\frac{r + \sum_{k = j}^{n - 1} f[k]}{n - j}⌋ - f[j] \\ 
  &= ⌊\frac{r + \sum_{k = j}^{n - 1} f[k]}{n - j}⌋
\end{aligned}
$$

由已知二式：
$$
f[j - 1](n - j + 1) - \sum_{k = j - 1}^{n - 1}f[k] > r \\
r + \sum_{k = j - 1}^{n - 1}f[k] < f[j - 1](n - j + 1)  \\ 
r + \sum_{k = j}^{n - 1}f[k] < f[j - 1](n - j + 1) - f[j - 1] = f[j - 1](n - j) \\ 
$$

故知：
$$
f[j] + ⌊\frac{r'}{n - j}⌋ < ⌊f[j - 1]⌋ = f[j - 1]
$$

Q.E.D